internal/examples/semantics/precedence.go
@@ -1,30 +1,30 @@
 package semantics
 
-func failing_testOrCompareSimple() bool {
+func testOrCompareSimple() bool {
 	if 3 > 4 || 4 > 3 {
 		return true
 	}
 	return false
 }
 
-func failing_testOrCompare() bool {
+func testOrCompare() bool {
 	var ok = true
 	if !(3 > 4 || 4 > 3) {
 		ok = false
 	}
-	if 3 > 4 || 2 > 3 {
+	if 4 < 3 || 2 > 3 {
 		ok = false
 	} else {
 	}
 	return ok
 }
 
-func failing_testAndCompare() bool {
+func testAndCompare() bool {
 	var ok = true
 	if 3 > 4 && 4 > 3 {
 		ok = false
 	}
-	if 4 > 3 || 3 > 2 {
+	if 4 > 3 || 2 < 3 {
 	} else {
 		ok = false
 	}
